VST-introduction/verif_simple_kfree_file_v2.v
@@ -165,7 +165,6 @@ Definition freerange_no_loop_no_add_1_spec :=
          PROP ()
          RETURN ()
          SEP (
-            (*denote_tc_test_order new_head pa_end **)
             if pointer_le_bool (Vptr b (Ptrofs.add p (Ptrofs.repr (PGSIZE)))) pa_end then
                (freelistrep sh (S n) (Vptr b p) *
                data_at sh t_struct_kmem (Vint (Int.repr xx), (Vptr b p)) (gv _kmem))
@@ -176,11 +175,78 @@ Definition freerange_no_loop_no_add_1_spec :=
                data_at sh t_struct_kmem (Vint (Int.repr xx), original_freelist_pointer) (gv _kmem)))
          ).
 
+(************** while loop ***************)
+Definition while_1_5_spec : ident * funspec :=
+    DECLARE _while_1_5
+    WITH b_n_init:block, p_n_init:ptrofs, b_s_init:block, p_s_init:ptrofs
+    PRE [  tptr tvoid, tptr tvoid ]
+        PROP (
+                0 <= Ptrofs.unsigned p_s_init <= Ptrofs.unsigned p_n_init /\
+                Z.add (Ptrofs.unsigned p_n_init) PGSIZE <= Int.max_signed /\ 
+                Z.add (Ptrofs.unsigned p_s_init) PGSIZE <= Int.max_signed 
+            ) (* the highest number is s + PGSIZE when it fails. The highest s + PGSIZE when it succeeds is n, so the highest after this is n + PGSIZE*)
+        PARAMS (Vptr b_s_init p_s_init; Vptr b_n_init p_n_init)
+        SEP (denote_tc_test_order ((Vptr b_s_init (Ptrofs.add p_s_init (Ptrofs.repr (PGSIZE))))) (Vptr b_n_init p_n_init))
+    POST [ tint ]
+    EX c:Z, EX p_s_final:ptrofs,
+        PROP (
+            Ptrofs.unsigned p_s_final = Z.add (Ptrofs.unsigned p_s_init) (Z.mul c PGSIZE) /\ 
+            0 <= c /\ 
+            (Ptrofs.unsigned p_s_final) <= (Ptrofs.unsigned p_n_init) /\ 
+            (Ptrofs.unsigned p_n_init) < Z.add (Ptrofs.unsigned p_s_final) PGSIZE
+            )
+        RETURN (Vint (Int.repr (c)))
+        SEP ((*denote_tc_test_order ((Vptr b_s_init (Ptrofs.add p_s_final (Ptrofs.repr (PGSIZE))))) (Vptr b_n_init p_n_init)*)).
+
+(*Definition freerange_while_loop_spec : ident * funspec :=
+DECLARE _freerange_while_loop
+WITH b_n_init:block, p_n_init:ptrofs, b_s_init:block, p_s_init:ptrofs, sh : share, original_freelist_pointer : val, xx : Z, gv : globals, n:nat
+PRE [  tptr tvoid, tptr tvoid ]
+      PROP (
+            0 <= Ptrofs.unsigned p_s_init <= Ptrofs.unsigned p_n_init /\
+            Z.add (Ptrofs.unsigned p_n_init) PGSIZE <= Int.max_signed /\ 
+            Z.add (Ptrofs.unsigned p_s_init) PGSIZE <= Int.max_signed /\
+            
+            writable_share sh /\ 
+            is_pointer_or_null original_freelist_pointer
+
+         ) (* the highest number is s + PGSIZE when it fails. The highest s + PGSIZE when it succeeds is n, so the highest after this is n + PGSIZE*)
+      PARAMS (Vptr b_s_init p_s_init; Vptr b_n_init p_n_init)
+      SEP (denote_tc_test_order ((Vptr b_s_init (Ptrofs.add p_s_init (Ptrofs.repr (PGSIZE))))) (Vptr b_n_init p_n_init) &&
+            (freelistrep sh n original_freelist_pointer *
+            (!! malloc_compatible (sizeof t_run) (Vptr b_s_init p_s_init) &&
+            data_at sh (t_run) nullval (Vptr b_s_init p_s_init) *
+            data_at sh t_struct_kmem (Vint (Int.repr xx), original_freelist_pointer) (gv _kmem) ))
+      )
+POST [ tint ]
+EX c:Z, EX p_s_final:ptrofs,
+      PROP (
+         Ptrofs.unsigned p_s_final = Z.add (Ptrofs.unsigned p_s_init) (Z.mul c PGSIZE) /\ 
+         0 <= c /\ 
+         (Ptrofs.unsigned p_s_final) <= (Ptrofs.unsigned p_n_init) /\ 
+         (Ptrofs.unsigned p_n_init) < Z.add (Ptrofs.unsigned p_s_final) PGSIZE
+         )
+      RETURN (Vint (Int.repr (c)))
+      SEP ((*denote_tc_test_order ((Vptr b_s_init (Ptrofs.add p_s_final (Ptrofs.repr (PGSIZE))))) (Vptr b_n_init p_n_init)*)
+            if pointer_le_bool (Vptr b (Ptrofs.add p (Ptrofs.repr (PGSIZE)))) pa_end then
+               (freelistrep sh (S n) (Vptr b p) *
+               data_at sh t_struct_kmem (Vint (Int.repr xx), (Vptr b p)) (gv _kmem))
+            else
+               (freelistrep sh n original_freelist_pointer *
+               (!! malloc_compatible (sizeof t_run) (Vptr b p) &&
+               data_at sh (t_run) nullval (Vptr b p) *
+               data_at sh t_struct_kmem (Vint (Int.repr xx), original_freelist_pointer) (gv _kmem)))
+      ).*)
+     
+
+
 
 (************************ Gprog  *************************)
 Definition Gprog : funspecs := [
    kfree1_freelist_spec;
-   freerange_no_loop_no_add_spec
+   freerange_no_loop_no_add_spec;
+   freerange_no_loop_no_add_1_spec;
+   while_1_5_spec
 ].
 
 
@@ -286,3 +352,98 @@ forward_if.
         rewrite e2 in e1. inversion e1.
       + apply andp_left2. entailer!.
 Qed.
+
+Lemma ptrofs_add_simpl :
+  forall a,
+    0 <= Ptrofs.unsigned a + PGSIZE < Ptrofs.modulus ->
+    Ptrofs.unsigned (Ptrofs.add a (Ptrofs.repr PGSIZE)) =
+    Ptrofs.unsigned a + PGSIZE.
+Proof.
+  intros.
+  unfold Ptrofs.add.
+  rewrite Ptrofs.unsigned_repr.
+  - rewrite Ptrofs.unsigned_repr; auto.
+    unfold PGSIZE; try rep_lia.
+  - destruct H; assert (Ptrofs.unsigned (Ptrofs.repr PGSIZE) = PGSIZE). { apply Ptrofs.unsigned_repr. unfold PGSIZE; try rep_lia. } split.
+    + rewrite H1; auto.
+    + rewrite H1; auto. try rep_lia.
+Qed. 
+
+Lemma body_while_1_5: semax_body Vprog Gprog f_while_1_5 while_1_5_spec.
+Proof. start_function. repeat forward.
+forward_while
+ (EX c_tmp: Z, EX p_s_tmp:ptrofs,
+   PROP  (
+    Ptrofs.unsigned p_s_tmp = Z.add (Ptrofs.unsigned p_s_init) (Z.mul c_tmp PGSIZE) /\ 
+    0 <= c_tmp /\
+    c_tmp <= Int.max_signed /\
+    Ptrofs.unsigned p_s_tmp <= Ptrofs.unsigned p_n_init
+   )
+   LOCAL (
+    temp _c (Vint (Int.repr c_tmp));
+    temp _pa_start (Vptr b_s_init p_s_tmp);
+    temp _pa_end (Vptr b_n_init p_n_init)
+    )
+   SEP (denote_tc_test_order ((Vptr b_s_init (Ptrofs.add p_s_tmp (Ptrofs.repr (PGSIZE))))) (Vptr b_n_init p_n_init))).
+
+   - EExists; EExists; entailer. 
+   - entailer!. unfold PGSIZE. entailer.
+   -repeat forward.
+    +entailer!. destruct H0. destruct H1. destruct H2.
+     split; try rep_lia.
+     apply Z.le_trans with (m := Ptrofs.unsigned p_s_init + c_tmp * PGSIZE + PGSIZE); try rep_lia.
+     assert (Ptrofs.unsigned p_s_init + c_tmp * PGSIZE + PGSIZE = Ptrofs.unsigned p_s_init + (c_tmp + 1) * PGSIZE) by rep_lia.
+     rewrite H4.
+     destruct c_tmp; try contradiction; try discriminate; unfold PGSIZE; auto; try rep_lia. 
+    + Exists (c_tmp + 1, Ptrofs.add p_s_tmp (Ptrofs.repr PGSIZE)). entailer!.
+        * split.
+            -- destruct H0. 
+                assert (Ptrofs.unsigned p_s_init + (c_tmp + 1) * PGSIZE = Ptrofs.unsigned p_s_init + (c_tmp) * PGSIZE + PGSIZE); try rep_lia.
+                rewrite H2.
+                assert (Ptrofs.unsigned p_s_init + c_tmp * PGSIZE + PGSIZE =  Ptrofs.unsigned p_s_tmp + PGSIZE); try rep_lia.
+                rewrite H3.
+                apply ptrofs_add_simpl; split; try rep_lia.
+                apply Z.add_nonneg_nonneg; unfold PGSIZE; try rep_lia.
+            -- split; try rep_lia. split; try rep_lia.
+                (* fix : c_tmp + 1 <= Int.max_signed*)
+                ++ apply Z.le_trans with (m := Ptrofs.unsigned p_s_init + c_tmp * PGSIZE + PGSIZE); try rep_lia.
+                    assert (Ptrofs.unsigned p_s_init + c_tmp * PGSIZE + PGSIZE = Ptrofs.unsigned p_s_init + (c_tmp + 1) * PGSIZE) by rep_lia.
+                    rewrite H1.
+                    destruct c_tmp; try contradiction; try discriminate; unfold PGSIZE; auto; try rep_lia.
+                ++ 
+                destruct (sem_cmp_pp Cle (offset_val 4096 (Vptr b_s_init p_s_tmp)) (* find a solution for magic number 4096 *)
+                (Vptr b_n_init p_n_init)) eqn:e; try contradiction; try discriminate.
+                destruct v; try discriminate; try contradiction.
+                assert (i = Int.zero \/ i = Int.one). {
+                    apply cmp_le_is_either_0_or_1 with (p:= (offset_val PGSIZE (Vptr b_s_init p_s_tmp))) (q:=(Vptr b_n_init p_n_init) ); auto.
+                }
+                destruct H1; try contradiction; try discriminate.
+                ** subst; try contradiction; try discriminate.
+                ** rewrite H1 in e. 
+                    unfold sem_cmp_pp in e; simpl in e. destruct (eq_block b_s_init b_n_init); try discriminate; try contradiction.
+                    subst. destruct ((negb (Ptrofs.ltu p_n_init (Ptrofs.add p_s_tmp (Ptrofs.repr 4096))))) eqn:e1; try discriminate; try contradiction.
+                    unfold negb in e1. destruct (Ptrofs.ltu p_n_init (Ptrofs.add p_s_tmp (Ptrofs.repr 4096))) eqn:e2; try discriminate; try contradiction.
+                    unfold Ptrofs.ltu in e2. destruct (zlt (Ptrofs.unsigned p_n_init) (Ptrofs.unsigned (Ptrofs.add p_s_tmp (Ptrofs.repr 4096)))) eqn: e3; try contradiction; try discriminate.
+                    unfold PGSIZE. try rep_lia.
+        * admit. (* fix denote_tc_test_order..*)
+    - forward. Exists c_tmp. Exists p_s_tmp. entailer!. 
+        split; try rep_lia. 
+        destruct (sem_cmp_pp Cle (offset_val 4096 (Vptr b_s_init p_s_tmp)) (* find a solution for magic number 4096 *)
+        (Vptr b_n_init p_n_init)) eqn:e; try contradiction; try discriminate.
+        destruct v; try discriminate; try contradiction.
+        assert (i = Int.zero \/ i = Int.one). {
+            apply cmp_le_is_either_0_or_1 with (p:= (offset_val PGSIZE (Vptr b_s_init p_s_tmp))) (q:=(Vptr b_n_init p_n_init) ); auto.
+        }
+        destruct H1.
+        2: { subst. try contradiction; try discriminate. }
+        subst.
+        unfold sem_cmp_pp in e. simpl in e. destruct (eq_block b_s_init b_n_init); try discriminate; try contradiction.
+        destruct ((Some (negb (Ptrofs.ltu p_n_init (Ptrofs.add p_s_tmp (Ptrofs.repr 4096)))))) eqn:e1; try discriminate; try contradiction.
+        destruct b; try discriminate; try contradiction.
+        unfold negb in e1; unfold Ptrofs.ltu in e1. destruct (zlt (Ptrofs.unsigned p_n_init) (Ptrofs.unsigned (Ptrofs.add p_s_tmp (Ptrofs.repr 4096)))) eqn:e2; try discriminate; try contradiction.
+        assert (Ptrofs.unsigned (Ptrofs.add p_s_tmp (Ptrofs.repr PGSIZE)) = Ptrofs.unsigned p_s_tmp + PGSIZE). {
+            apply ptrofs_add_simpl; split; try rep_lia. apply Z.add_nonneg_nonneg; unfold PGSIZE; try rep_lia.
+        }
+        rewrite <- H1. unfold PGSIZE; apply l.
+Admitted.
+
